Update compiler to produce error messages.

Compiler.v
@@ -1,6 +1,6 @@
 Require Import List CSet.
-Require Import Util AllInRel IL ILRaise EnvTy ParamsMatch RegAlloc RenameApart Sim.
-Require Coherence ILIToILF Liveness ParallelMove ILN LivenessAnalysis CoherenceAlgo.
+Require Import Util AllInRel IL ILRaise EnvTy ParamsMatch RegAlloc RenameApart Sim Status.
+Require Coherence ILIToILF Liveness ParallelMove ILN LivenessAnalysis CoherenceAlgo RegAllocAlgo.
 
 Require Import ExtrOcamlBasic.
 Require Import ExtrOcamlZBigInt.
@@ -11,9 +11,9 @@ Set Implicit Arguments.
 
 Section Compiler.
 
-Hypothesis allocation_oracle : forall {s:stmt} {G G':set var}, Coherence.ssa G s G' -> var -> var.
+Hypothesis allocation_oracle : stmt -> ann (set var) -> (var -> var) -> status (var -> var).
 Hypothesis ssa_construction : stmt -> ann (option (set var)) * ann (list var).
-Hypothesis parallel_move : var -> list var -> list var -> option (list(list var * list var)).
+Hypothesis parallel_move : var -> list var -> list var -> (list(list var * list var)).
 Hypothesis first : ann (set var) -> ( ann (set var) -> ann (set var) * bool) -> ann (set var).
 
 Definition livenessAnalysis (s:stmt) :=
@@ -22,72 +22,86 @@ Definition livenessAnalysis (s:stmt) :=
 Definition additionalArguments s lv :=
   fst (CoherenceAlgo.computeParameters nil nil s lv).
 
-Definition toILF (ili:stmt) (lv:ann(set var)) : option IL.stmt :=
+Definition toILF (ili:stmt) (lv:ann (set var)) : status IL.stmt :=
   if [Liveness.live_sound nil ili lv] then
     let additional_arguments := additionalArguments ili lv
-    in if [ILIToILF.trs nil nil (freeVars ili) ili lv additional_arguments] then
-         Some (ILIToILF.compile nil ili additional_arguments)
-       else None
-    else None.
+    in if [ILIToILF.trs nil nil ili lv additional_arguments] then
+         Success (ILIToILF.compile nil ili additional_arguments)
+       else Error ("Additional Arguments insufficient")
+    else Error ("Liveness unsound").
 
 
-Definition fromILF (s:stmt) : option stmt :=
+Definition fromILF (s:stmt) : status stmt :=
   let s_renamed_apart := rename_apart s
-  in let ϱ := allocation_oracle (rename_apart_ssa s)
-     in let lv := livenessAnalysis s_renamed_apart
-        in if [Liveness.live_sound nil s_renamed_apart lv
-               /\ getAnn lv ⊆ freeVars s 
-               /\ agree_on (getAnn lv) ϱ id
-               /\ locally_inj ϱ s_renamed_apart lv ] then
-             let s_allocated := rename ϱ s_renamed_apart in
-             mdo s_lowered <- ParallelMove.lower parallel_move nil s_allocated (Liveness.live_rename ϱ lv) ;
-             Some s_lowered
-           else
-             None.
+  in let lv := livenessAnalysis s_renamed_apart in
+     if [Liveness.live_sound nil s_renamed_apart lv
+         /\ getAnn lv ⊆ freeVars s] then
+       sdo ϱ <- allocation_oracle s_renamed_apart lv id;
+       if [agree_on (getAnn lv) ϱ id
+           /\ locally_inj ϱ s_renamed_apart lv ] then
+         let s_allocated := rename ϱ s_renamed_apart in
+         let s_lowered := ParallelMove.lower parallel_move nil s_allocated (mapAnn (lookup_set ϱ) lv) in
+         s_lowered
+       else
+         Error "Register allocation not injective."
+     else
+       Error "Liveness unsound.".
 
-Lemma toILF_correct ili s E
+Lemma toILF_correct ili alv s E
   : params_match (nil: list I.block) ili
-   -> toILF ili = Some s
+   -> toILF ili alv = Success s
    -> sim (nil:list I.block, E, ili) (nil:list F.block, E, s).
 Proof.
-  intros. unfold toILF in H0. destruct (ssa_construction ili); intros. 
-  destruct if in H0; isabsurd; monad_inv H0. 
+ intros. unfold toILF in H0; simpl in *.
+  Opaque Liveness.live_sound_dec.
+  Opaque ILIToILF.trs_dec.
+  destruct if in H0.
+  destruct if in H0; isabsurd. inv H0.
   refine (sim_trans (ILIToILF.trsR_sim _) (sim_sym (Coherence.srdSim_sim _))).
   econstructor; eauto using AIR4; eauto; try reflexivity; isabsurd.
   econstructor; eauto 30 using ILIToILF.compile_typed, agree_on_refl, AIR2; isabsurd.
-  split; isabsurd. 
+  split; isabsurd.
   destruct H; eauto using (ILIToILF.compile_params_match t H).
+  instantiate (1:=nil).
+  admit.
+  isabsurd.
 Qed.
 
 Lemma fromILF_correct (s s':stmt) E
   : params_match nil s
-  -> fromILF s = Some s' 
+  -> fromILF s = Success s' 
   -> sim (nil:list F.block, E, s) (nil:list I.block, E, s').
 Proof.
-  unfold fromILF; intros. destruct if in H0; dcr; isabsurd.
-  monad_inv H0; dcr.
+  unfold fromILF; intros.
+  destruct if in H0; dcr; isabsurd.
+  monadS_inv H0; dcr. destruct if in EQ0.
   eapply sim_trans with (σ2:=(nil:list F.block, E, rename_apart s)). 
   eapply (@Alpha.alphaSim_sim (nil, E, s) (nil, E, rename_apart s)).
   econstructor; eauto using AIR3, Alpha.envCorr_idOn_refl. 
   eapply Alpha.alpha_sym. eapply rename_apart_alpha.
   eapply sim_trans with (σ2:=(nil:list F.block, E, 
-    rename (allocation_oracle (rename_apart_ssa s)) (rename_apart s))). 
+    rename x (rename_apart s))).
   eapply Alpha.alphaSim_sim. econstructor; eauto using AIR3.
   eapply ssa_locally_inj_alpha; eauto.
   eapply rename_apart_ssa; eauto; eapply lookup_set_on_id; try reflexivity.
-  instantiate (1:=id). eapply agree_on_inverse_on; eauto; intuition.
+  eapply a.
+  instantiate (1:=id). admit.
   split. simpl. eapply (rename_apart_parameters_match (L:=nil)); isabsurd; eauto.
-  simpl. eapply H. isabsurd. 
-  hnf; intros. cbv in H4; subst. rewrite H4; eauto.
+  simpl. eapply H. isabsurd.
+  hnf; intros. cbv in H3; subst. rewrite H3; eauto.
   refine (sim_trans (Coherence.srdSim_sim _) (ParallelMove.pmSim_sim _)).
   econstructor; isabsurd. eapply rename_ssa_srd; eauto.
-  eapply rename_apart_ssa; eauto.
+  eapply rename_apart_ssa; eauto. eapply a.
   eapply I. econstructor. eapply rename_params_match with (L:=nil).
   eapply rename_apart_params_match; eauto.
   eapply agree_on_refl.
-  econstructor; eauto using AIR3; isabsurd. 
-  eapply (@Liveness.live_rename_sound nil); eauto. 
+  eapply (@Liveness.live_rename_sound nil); eauto.
+  instantiate (1:=parallel_move). 
+  econstructor; try eapply EQ0.
+  eapply (@Liveness.live_rename_sound nil); eauto.
+  constructor.
   reflexivity.
+  congruence.
 Qed.
 
 End Compiler.
